tests/cpp2v-parser/test_delegating_init.cpp
@@ -1,0 +1,4 @@
+struct Foo {
+    Foo() {};
+    Foo(int):Foo() {}
+};
